Actus/Trace.lean
@@ -1,9 +1,20 @@
 import Actus.Types
+import Actus.Logic
+open MetricTemporalSemantics
 
-namespace Trace
-  structure TraceEntry (E : Type) where
-    e : E
-    t : Time.Timestamp
+structure TraceEntry (E : Type) where
+  e : E
+  t : Time.Timestamp
 
-  def T (E : Type) := E |> TraceEntry |> List
-end Trace
+def TraceEntry.map {E F : Type} (f : E -> F) (te : TraceEntry E) : TraceEntry F :=
+  { e := f te.e, t := te.t }
+
+instance : Functor TraceEntry where
+  map := TraceEntry.map
+
+def Trace (E : Type) := E |> TraceEntry |> List
+
+def Trace.toModel (trace : Trace E) : Model E :=
+  fun t => trace.find? (fun entry => entry.t = t) |>.map (·.e)
+
+-- def Trace.valid (E : Type) (trace : Trace E) (contract : MetricTemporal.Proposition E): Prop :=
