comms/whitepaper/source.typ
@@ -1,1 +1,22 @@
-#+title: Finance as a Reactive System
+#set heading(numbering: "1.")
+
+#let title = [Can Finance be Formally Verified? Notes from Reactive Systems]
+#let abstract = [#lorem(80)]
+#align(center, text(17pt)[
+  *#title*
+])
+#grid(
+  columns: (1fr),
+  align(center)[
+    Quinn Dougherty \
+    Casper Association \
+    #link("mailto:quinn@casper.network")
+  ],
+)
+
+#align(center)[
+  #set par(justify: false)
+  *Abstract* \
+  #abstract
+]
+Finance as a Reactive System
