nix/comms/whitepaper/default.nix
@@ -1,13 +1,16 @@
 { self, pkgs }:
 pkgs.stdenv.mkDerivation {
   name = "mtl-actus-whitepaper";
-  buildInputs = [ pkgs.typst ];
-  src = "${self}/comms/whitepaper/";
+  buildInputs = [
+    pkgs.pandoc
+    pkgs.texliveSmall
+  ];
+  src = "${self}/comms/whitepaper";
   buildPhase = ''
-    typst compile source.typ
+    pandoc -t latex -f org $src/source.org -o whitepaper.pdf
   '';
   installPhase = ''
     mkdir -p $out
-    cp source.pdf $out/whitepaper.pdf
+    cp -r whitepaper.pdf $out
   '';
 }
