nix/comms/whitepaper/typst.nix
@@ -1,0 +1,13 @@
+{ self, pkgs }:
+pkgs.stdenv.mkDerivation {
+  name = "mtl-actus-whitepaper";
+  buildInputs = [ pkgs.typst ];
+  src = "${self}/comms/whitepaper/";
+  buildPhase = ''
+    typst compile source.typ
+  '';
+  installPhase = ''
+    mkdir -p $out
+    cp source.pdf $out/whitepaper.pdf
+  '';
+}
